\unless\ifdefined\IsMainDocument
\documentclass[12pt]{article}
\usepackage{amsmath,amsthm,amssymb}
\newcommand{\Z}{\mathbb{Z}}
\newcommand{\IntPart}[1]{\left[ #1 \right]}
\newcommand{\val}[1]{\nu\left( #1 \right)}
\newcommand{\pval}[1]{\nu_p\left( #1 \right)}
\begin{document}
\fi

\textbf{Problem 4.7}: For $n \in \Z^+$ put $L(n) = \exp \psi(n)$.
\begin{enumerate}
\item For $k \in \Z^+$ show that
$$L(2k) \leq 2L(2k-1)$$
$$L(2k+1) \leq \binom{2k+1}{k+1} L(k+1) < 2^{2k} L(k+1)$$
\item Use (1) to show that $L(n) < 4^n$ i.e. $\psi(n) < n \log 4$ for $n \in \Z^+$.
\end{enumerate}

\begin{proof}
\begin{enumerate}
\item Evidently, $2L(2k-1)$ is divisible by $1, 2, ..., 2k - 1$ and is also divisible by $2k$ since $k | L(2k-1)$. Thus, $2L(2k-1)$ is a common multiple of $\{1, 2, ..., 2k\}$ and so it is $\geq L(2k)$ which is the least common multiple of those numbers.

To prove the second inequality, we show that the quotient
$$\frac{L(2k+1)}{L(k+1)} \text{ divides } \binom{2k+1}{k+1}$$
by first observing that the quotient is square-free. This is easy to see as its logarithm is:
$$\psi(2k+1) - \psi(k+1) = \sum_{k + 1 < p^\alpha \leq 2k+1} \log p$$
and any prime $p$ can only participate once in the sum: For we then have $2(k+1) < 2 p^\alpha$ and so $p^\alpha$ is the maximum power of $p$ not exceeding $2k+1$. But if $p$ is such a prime then it divides $\binom{2k+1}{k+1}$ by $p$-adic valuation:
$$\pval{\binom{2k+1}{k+1}} \geq \underbrace{\IntPart{\frac{2k+1}{p^\alpha}}}_{1} - \underbrace{\IntPart{\frac{k+1}{p^\alpha}}}_{0} - \underbrace{\IntPart{\frac{k}{p^\alpha}}}_{0} = 1.$$

The remaining inequality is simple:
\begin{align*}
2^{2k+1} &= (1 + 1)^{2k+1}\\
&= \sum_{j = 0}^{2k+1} \binom{2k + 1}{j}\\
&> \binom{2k+1}{k} + \binom{2k+1}{k+1}\\
&= 2 \binom{2k+1}{k+1}.
\end{align*}

\item Finally, we prove $L(n) < 4^n$ by induction. The base case $n = 1$ is evident. Suppose that the inequality is true for all $n < k$ and we show it is true for $n = k$.
\begin{itemize}
\item If $k = 2 \ell$ is even then
$$L(k) = L(2\ell) \leq 2 L(2\ell - 1) < 2 (4^{2\ell - 1}) < 4^{2\ell} = 4^k.$$
\item If $k = 2 \ell + 1$ is odd then
$$L(k) = L(2\ell+1) < 2^{2\ell} L(\ell + 1) < 4^{\ell} (4^{\ell + 1}) = 4^{2\ell + 1} = 4^k.$$
\end{itemize}
\end{enumerate}
\end{proof}

\unless\ifdefined\IsMainDocument
\end{document}
\fi
