\unless\ifdefined\IsMainDocument
\documentclass[12pt]{article}
\usepackage{amsmath,amsthm,amssymb}

\begin{document}
\fi

\textbf{Problem 5.9}: Show that
$$Q(x) := \sum_{n \leq x} |\mu(n)| = 6 \pi^{-2} x + o(\sqrt{x}).$$

\begin{proof}
Write $|\mu| = 1 * f$ as in Lemma 3.4 (actually $f = 1_S^{*-1}$ as seen in problem 5.6) and note that the summatory function of $f$ is precisely $M(\sqrt{x})$. Therefore
\begin{align*}
Q(x) &= \int_{1^-}^x dN(t) * dM(\sqrt{t})\\
&= \int_{1^-}^x N\left(\frac x t\right) \; dM(\sqrt{t})\\
&= \int_{1^-}^{\sqrt x} N\left(\frac{x}{u^2}\right) \; dM(u) &\text{by change of variable } u = \sqrt{t}\\
&= \int_{1^-}^{\sqrt x} \frac{x}{u^2} \; dM(u) + \int_{1^-}^{\sqrt x} \left\{ N\left(\frac{x}{u^2}\right) - \frac{x}{u^2} \right\} \; dM(u) &\text{the usual trick}
\end{align*}

We can write $N\left(\frac{x}{u^2}\right) - \frac{x}{u^2} = N\left(\left\{\frac{\sqrt x}{u}\right\}^2\right) - \left\{\frac{\sqrt x}{u}\right\}^2$ to recognize the second integral
$$\int_{1^-}^{\sqrt x} \left\{ N\left(\frac{x}{u^2}\right) - \frac{x}{u^2} \right\} \; dM(u) = \int_{1^-}^{\sqrt x} dG * dM$$
where $G(t) = N(t^2) - t^2$. The same trick in Corollary 5.9 applies here: $|G(t)| \leq 1$ and $\int_{1^-}^{\infty} 1 \cdot u^{-2} du < \infty$ so $\int_{1^-}^{x} dG * dM = o(x)$ from the fact that $M(x) = o(x)$ by Theorem 5.9. This implies that the above integral is $o(\sqrt x)$. The first integral has the familiar treatment:
\begin{align*}
\int_{1^-}^{\sqrt x} \frac{x}{u^2} \; dM(u) &= x \left\{ \int_{1^-}^{\infty} - \int_{\sqrt x}^{\infty} \right\} \frac{1}{u^2} \; dM(u)\\
&= 6 \pi^{-2} x - x \int_{\sqrt x}^{\infty} \frac{1}{u^2} \; dM(u)\\
&= 6 \pi^{-2} x - x \left\{ \left. \frac{M(u)}{u^2} \right|_{\sqrt x}^{\infty} - \int_{\sqrt x}^{\infty} M(u) d(u^{-2}) \right\}\\
&= 6 \pi^{-2} x - x \left\{ -\frac{M(\sqrt x)}{x} + 2 \int_{\sqrt x}^{\infty} M(u) u^{-3} du \right\} &\text{ as } M(x) = o(x)\\
&= 6 \pi^{-2} x + M(\sqrt{x}) - 2 x \int_{\sqrt x}^{\infty} o(u^{-2}) du &\text{ as } M(x) = o(x)\\
&= 6 \pi^{-2} x + o(\sqrt{x}) &\text{ as } M(x) = o(x)
\end{align*}
and
$$\int_{\sqrt x}^{\infty} o(u^{-2}) du = o\left( \left. -\frac{1}{u} \right|_{\sqrt x}^{\infty} \right) = o(x^{-1/2}).$$
\end{proof}

\unless\ifdefined\IsMainDocument
\end{document}
\fi
